change lt to le

Matroids/Sort.lean
@@ -6,4 +6,4 @@ import Mathlib.Data.List.Sort
 list is greater. Its criteria for determining the greater list is whichever list generates a greater
 number first-/
 def List.sort {X : Type*} [LinearOrder X] (l : List X) : List X :=
-   l.mergeSort (· < · )
+   l.mergeSort (· ≤ · )
