Matroids/Verification/PartialMatroid.lean
@@ -49,7 +49,7 @@ lemma augment_normalized (l : List Nat) (A : PartialMatroid)
     simp (config := {decide := true})
     have h := hA 0 1
     simp (config := {decide := true}) at h
-    rw [← List.mem_mergeSort (le := (· < ·))]
+    rw [← List.mem_mergeSort (le := (· ≤ ·))]
     simp [sort]
     right
     apply h
@@ -58,7 +58,7 @@ lemma augment_normalized (l : List Nat) (A : PartialMatroid)
     simp (config := {decide := true})
     have h := hA 0 2
     simp (config := {decide := true}) at h
-    rw [← List.mem_mergeSort (le := (· < ·))]
+    rw [← List.mem_mergeSort (le := (· ≤ ·))]
     simp [sort]
     right
     apply h
@@ -67,7 +67,7 @@ lemma augment_normalized (l : List Nat) (A : PartialMatroid)
     simp (config := {decide := true})
     have h := hA 0 3
     simp (config := {decide := true}) at h
-    rw [← List.mem_mergeSort (le := (· < ·))]
+    rw [← List.mem_mergeSort (le := (· ≤ ·))]
     simp [sort]
     right
     apply h
@@ -78,7 +78,7 @@ lemma augment_normalized (l : List Nat) (A : PartialMatroid)
     simp (config := {decide := true})
     have h := hA 1 2
     simp (config := {decide := true}) at h
-    rw [← List.mem_mergeSort (le := (· < ·))]
+    rw [← List.mem_mergeSort (le := (· ≤ ·))]
     simp [sort]
     right
     apply h
@@ -87,7 +87,7 @@ lemma augment_normalized (l : List Nat) (A : PartialMatroid)
     simp (config := {decide := true})
     have h := hA 1 3
     simp (config := {decide := true}) at h
-    rw [← List.mem_mergeSort (le := (· < ·))]
+    rw [← List.mem_mergeSort (le := (· ≤ ·))]
     simp [sort]
     right
     apply h
@@ -151,28 +151,24 @@ lemma augment_lawful (l : List Nat) (A : PartialMatroid)
     unfold augment
     simp
     unfold sort
-    have h_nodup : Nodup (l :: A.matroid) := by
+    apply (sorted_mergeSort' (l :: A.matroid)).lt_of_le
+    apply (mergeSort_perm ..).symm.nodup
+    simp
+    constructor
+    · contrapose l_not_nearlySame_as_matroid
+      simp at l_not_nearlySame_as_matroid
+      rw[List.forall_iff_forall_mem]
+      simp
+      use l
+      constructor
+      · exact l_not_nearlySame_as_matroid
+      · exact NearlySame.refl
+    · have h := hA.pairwise_not_nearlySame
+      apply List.Pairwise.nodup at h
+      · exact h
+      · refine { irrefl := ?_ }
         simp
-        constructor
-        · contrapose l_not_nearlySame_as_matroid
-          simp at l_not_nearlySame_as_matroid
-          rw[List.forall_iff_forall_mem]
-          simp
-          use l
-          constructor
-          · exact l_not_nearlySame_as_matroid
-          · exact NearlySame.refl
-        · have h := hA.pairwise_not_nearlySame
-          apply List.Pairwise.nodup at h
-          · exact h
-          · refine { irrefl := ?_ }
-            simp
-            apply NearlySame.refl
-    apply List.Sorted.lt_of_le
-    · rw [List.mergeSort_lt_eq_mergeSort_le h_nodup]
-      apply List.sorted_mergeSort''
-    · apply List.mergeSort_no_duplicates
-
+        apply NearlySame.refl
   pairwise_not_nearlySame := by
     unfold augment
     dsimp
