Matroids/Verification/Sort.lean
@@ -5,77 +5,6 @@ import Mathlib.Data.List.Sort
 
 open List
 
-/--mergeSort with the less than relation has no duplicates-/ -- Wrong lemma, counterexample below
-lemma List.mergeSort_no_duplicates [PartialOrder α] {l : List α} [DecidableRel ((· : α) < ·)]:
-   Nodup (mergeSort l (· < ·)) :=
-
-  sorry
-
-
-
--- lemma List.split_of_sublist {α : Type*} {l : List α} :
---     List.Sublist (l.split).1 l ∧ List.Sublist (l.split).2 l:= by
---   match l with
---   | [] => simp
---   | a :: l =>
---     unfold split
---     simp
---     have ih := List.split_of_sublist (l := l)
---     constructor
---     · exact ih.2
---     · apply List.sublist_cons_of_sublist
---       exact ih.1
-
-
-/- Paused for the moment, we will focus on proving sorted_mergeSort for the less than relationship-/
-lemma List.mergeSort_lt_eq_mergeSort_le [LinearOrder α] {l : List α}
-    (h_nodup : l.Nodup):
-    mergeSort l (· < ·) = mergeSort l (· ≤ ·)  := by
-  match l with
-  | [] => simp
-  | [a] => simp
-  | a :: b :: l =>
-    unfold mergeSort
-    simp
-    -- have ha1 : List.Sublist (a :: (split l).1) (a :: b :: l) := by
-    --   apply List.Sublist.cons_cons
-    --   apply List.sublist_cons_of_sublist
-    --   apply List.split_of_sublist.1
-    -- have hb2 : List.Sublist (b :: (split l).2) (a :: b :: l) := by
-    --   apply List.sublist_cons_of_sublist
-    --   apply List.Sublist.cons_cons
-    --   apply List.split_of_sublist.2
-    -- have ha := List.Nodup.sublist ha1 h_nodup
-    -- have hb := List.Nodup.sublist hb2 h_nodup
-    -- have iha := List.mergeSort_lt_eq_mergeSort_le ha
-    -- have ihb := List.mergeSort_lt_eq_mergeSort_le hb
-    -- simp_rw[iha,ihb]
-    -- unfold merge
-    -- have : (split l = ((split l).1, (split l).2)) := by simp
-    -- have := perm_split this
-
-    -- simp at h_nodup
-    -- obtain ⟨hab, _, _⟩ := h_nodup
-    -- rw[or_iff_not_and_not] at hab
-    -- simp at hab
-    -- match mergeSort (fun x x_1 => x ≤ x_1) (a :: (split l).1), mergeSort (fun x x_1 => x ≤ x_1) (b :: (split l).2) with
-    -- | [], [] => simp
-    -- | [], l' => simp
-    -- | a :: l, [] => simp
-    -- | (x1 :: l1 as full1), (x2 :: l2 as full2)=>
-    --   simp
-
-    -- conv =>
-    --   lhs
-    --   arg 6
-    --   intro x1 x2 x3 x4
-      -- rw[lt_iff_le_and_ne (a := x1) (b := x3)]
-
-    sorry
-
-lemma List.mergeSort_lt_eq_mergeSort_le' [LinearOrder α] {l : List α}:
-    mergeSort l (· < ·) = mergeSort l (· ≤ ·) := by
-  sorry
 
 lemma List.not_mem_mergeSort (r : α → α → Bool) {l : List α} (h : a ∉ l) :
     a ∉ l.mergeSort r := by
@@ -94,25 +23,6 @@ lemma List.forall_mergeSort (r : α → α → Bool) {l : List α} {P : α → P
   apply List.Perm.symm
   apply List.mergeSort_perm
 
--- switch to library `List.sorted_mergeSort'` after
--- https://github.com/leanprover-community/mathlib4/pull/16902
-theorem List.sorted_mergeSort'' {α : Type u} (r : α → α → Prop) [DecidableRel r] [IsTotal α r]
-    [IsTrans α r] (l : List α) :
-    Sorted r (l.mergeSort fun (x1 x2 : α) => decide (r x1 x2)) :=
-  sorry
-
-/- PENDING theorem: If you have two different sorted lists and you run merge on them,
-then the result has to be sorted. Take a look at theorem Sorted.merge-/
-
-
-theorem sorted_mergeSort_lt [PartialOrder α] {l : List α} [DecidableRel ((· : α) < ·)] :
-    ∀ l : List α, Sorted (· < ·) (mergeSort l (· < ·))
-  | [] => by simp [mergeSort]
-  | [a] => by simp [mergeSort]
-  | a :: b :: l => by
-    simp [mergeSort]
-
-    sorry
 
 
 
@@ -140,16 +50,12 @@ lemma sort_flatten_map_sort {X : Type} [LinearOrder X] (L : List (List X)):
   sorry
 
 
+-- look up `List.eq_of_perm_of_sorted`
 lemma mergeSort_of_perm_eq {L₁ L₂ : List X} (P : X → X → Bool) (hL : L₁.Perm L₂) :
-    List.mergeSort L₁ P = List.mergeSort L₂ P := by
+    List.mergeSort L₁ P = List.mergeSort L₂ P :=
   sorry
 
 
 lemma mergeSort_sorted_list_X_Nat [LinearOrder X] (l : List (X × Nat)) :
-    (l.mergeSort (fun (x1, n1) (x2, n2) ↦ x1 < x2)).Sorted (fun (x1, _) (x2, _) ↦ x1 ≤ x2) := by sorry
-
-
-
-lemma mergeSort_lt_le_eq_List_X_Nat [LinearOrder X] (l : List (X × Nat)) :
-    l.mergeSort (fun (x1, n1) (x2, n2) ↦ x1 < x2) = l.mergeSort (fun (x1, n1) (x2, n2) ↦ x1 ≤ x2) := by
+    (l.mergeSort (fun (x1, n1) (x2, n2) ↦ x1 ≤ x2)).Sorted (fun (x1, _) (x2, _) ↦ x1 ≤ x2) := by
   sorry
